Vizing/new/Subfan.lean
@@ -1,14 +1,14 @@
 import Vizing.new.Fan
+import Vizing.new.TakeUntil
 
 set_option linter.dupNamespace false
 set_option push_neg.use_distrib true
 -- set_option trace.profiler true
 
-namespace Subfan
+namespace Fan
 open Graph
-open Nbhd
 open EdgeColoring
-open Fan
+open Aux
 
 /-
 
@@ -27,54 +27,70 @@ variable {n c : Nat} (G : Graph n) (C : EdgeColoring c G) (x y : Vertex n)
 def isSubfan (F1 F2 : Fan G C x y) :=
   F1.val.isPrefixOf F2.val
 
-/-
-
-If F is a strict subfan of G, there exists an element we can add to F
-to create a larger fan.
-
-That is, there is a vertex z adjacent to x such that the color of (x, z) is free on F.back.
-
-Prefix -> equal or there exists another element we can add
-
-That element is adjacent to
-
--/
-
 theorem maximalFan_spec : ∀ (F : Fan G C x y),
   isSubfan G C x y (maximalFan G C x y h) F →
   F.val = (maximalFan G C x y h).val := by
   intro F hF
   simp [isSubfan, ← Array.isPrefixOf_toList] at hF
   rcases (lt_or_eq_of_le (List.IsPrefix.length_le hF)) with hlt | heq
-  · exfalso
+  · have ⟨_, hF'⟩ := List.prefix_iff_getElem.mp hF
+    rw [List.prefix_iff_eq_append, List.drop_eq_getElem_cons hlt] at hF
     have hsize := (Array.size_pos_iff.mpr (maximalFan G C x y h).nonemptyAx)
-    have ⟨_, aux0⟩ := List.prefix_iff_getElem.mp hF
-
-    apply List.prefix_iff_eq_append.mp at hF
-    rw [List.drop_eq_getElem_cons hlt] at hF
-
-    have := F.colorAx
-    simp [colorAx] at this
-    specialize this ((maximalFan G C x y h).val.toList.length - 1) (by simp; apply Nat.sub_lt_sub_right hsize hlt)
-    simp at this;
-
-    have aux : (maximalFan G C x y h).val.size - 1 + 1 = (maximalFan G C x y h).val.size := by
-      apply Nat.sub_add_cancel hsize
-    simp_rw [aux] at this
-
-    specialize aux0 ((maximalFan G C x y h).val.toList.length - 1) (Nat.sub_one_lt (Nat.ne_zero_of_lt hsize))
-    simp at aux0
-    rw [← aux0] at this
-    
-
-    have := add_maximal G C x y (default G C x y h).val ((nbhd G x).val.erase y) (default G C x y h).nonemptyAx
-    simp [Array.back] at this
-    specialize this F.val[(maximalFan G C x y h).val.size] (by sorry )
-    simp_all [maximalFan, mkMaxFan]
+    specialize hF' ((maximalFan G C x y h).val.toList.length - 1)
+      (Nat.sub_one_lt (Nat.ne_zero_of_lt hsize))
+    have hcolor := F.colorAx ((maximalFan G C x y h).val.toList.length - 1)
+      (by simp; apply Nat.sub_lt_sub_right hsize hlt)
+    simp at hF' hcolor
+    simp_rw [Nat.sub_add_cancel hsize, ← hF'] at hcolor
+    contrapose! hcolor
+    simp [maximalFan]
+    apply mkMaxFan_maximal
+    all_goals simp_all only [maximalFan]
+    · apply (List.mem_erase_of_ne ?_).mpr
+      · apply F.nborsAx
+        apply Array.getElem_mem_toList
+      · simp_rw [← F.firstElemAx]
+        have hc := (maximalFan G C x y h).nonemptyAx
+        simp [maximalFan, ← F.firstElemAx] at hc
+        contrapose! hc
+        apply (List.Nodup.getElem_inj_iff F.nodupAx).mp at hc
+        exact Array.eq_empty_of_size_eq_zero hc
+    · have h := F.nodupAx
+      rw [← hF, List.nodup_middle] at h
+      apply List.Nodup.notMem at h
+      simp at h
+      exact h.left
   · apply Array.toList_inj.mp
+    apply Eq.symm
     apply List.IsPrefix.eq_of_length_le
     simp_all
-    sorry
-    exact Nat.le_of_eq heq
+    exact Nat.le_of_eq (Eq.symm heq)
 
-end Subfan
+def findSubfanWithColor (F : Fan G C x y) (a : Color c) : Fan G C x y where
+  val := takeUntil (a ∉ freeColorsOn G C ·) F.val
+  nborsAx := by
+    intro v hv
+    apply F.nborsAx
+    apply List.IsPrefix.mem hv
+    rw [← List.isPrefixOf_iff_prefix, Array.isPrefixOf_toList]
+    exact takeUntil_prefix (a ∉ freeColorsOn G C ·) F.val
+  nonemptyAx := by
+    simp [takeUntil]
+    exact F.nonemptyAx
+  firstElemAx := by
+    simp [takeUntil]
+    exact F.firstElemAx
+  colorAx := by
+    simp [colorAx, takeUntil]
+    intro i h
+    apply F.colorAx
+    simp_rw [← Nat.pred_eq_sub_one, ← Nat.pred_min_pred] at h
+    simp at h
+    exact h.right
+  nodupAx := by
+    apply List.Sublist.nodup ?_ F.nodupAx
+    apply List.IsPrefix.sublist
+    rw [← List.isPrefixOf_iff_prefix, Array.isPrefixOf_toList]
+    exact takeUntil_prefix (a ∉ freeColorsOn G C ·) F.val
+
+end Fan
