Vizing/new/TakeUntil.lean
@@ -1,0 +1,61 @@
+import Std
+import Mathlib.Data.List.Lemmas
+import Mathlib.Tactic
+
+/-
+
+Given an array A and a predicate p, takeUntil will return the prefix of A
+up to *and including* the first element that does not satisfy p.
+
+If every element in the array satisfies p, takeUntil p A = A.
+
+So, takeUntil p A = if takeWhile p A ≠ A then
+  takeWhile p A ++ A[(takeWhile p A).size] else
+  takeWhile p A
+
+-/
+
+namespace Aux
+
+def takeUntil {α : Type} [BEq α] [LawfulBEq α] (p : α → Bool) (A : Array α) :=
+  A.extract 0 (A.findIdx (!p ·) + 1)
+
+theorem takeUntil_prefix {α : Type} [BEq α] [LawfulBEq α] (p : α → Bool) (A : Array α) :
+  (takeUntil p A).isPrefixOf A := by
+  rw [takeUntil, ← Array.isPrefixOf_toList]
+  simp
+  exact List.take_prefix (Array.findIdx (fun x ↦ !p x) A + 1) A.toList
+
+theorem takeUntil_spec {α : Type} [BEq α] [LawfulBEq α]
+  (p : α → Bool) (A : Array α) (i : Fin (takeUntil p A).size) :
+  i < (takeUntil p A).size - 1 → p (takeUntil p A)[i] := by
+  intro h
+  by_cases ha : Array.findIdx (!p ·) A = A.size
+  · simp [takeUntil, ha]
+    have := Array.findIdx_eq_size.mp ha
+    simp at this; apply this
+    exact Array.mem_of_getElem rfl
+  · simp [takeUntil]
+    have aux : ∀ x ∈ A.takeWhile p, p x := by
+      rw [List.takeWhile_toArray]
+      simp only [Array.mem_toArray]
+      intro x h
+      apply List.mem_takeWhile_imp at h
+      assumption
+    apply aux
+    simp_rw [Array.takeWhile_eq_extract_findIdx_not]
+    apply Array.mem_extract_iff_getElem.mpr
+    use i
+    constructor
+    · simp_all
+      have := Array.getElem_extract i.isLt
+      simp only [zero_add, ← Fin.getElem_fin] at this
+      exact Eq.symm this
+    · simp_all [takeUntil]
+      rw [← Nat.pred_eq_sub_one, ← Nat.pred_min_pred] at h
+      simp at h
+      rcases h with ⟨l, r⟩
+      constructor
+      all_goals omega
+
+end Aux
