Vizing/new/Upstream.lean
@@ -2,7 +2,9 @@ import Mathlib.Data.List.Lemmas
 import Mathlib.Data.Finset.Card
 import Mathlib.Tactic
 
-theorem nodup_subset_eq_length_le {α : Type} [DecidableEq α] (L M : List α)
+namespace Aux
+
+theorem length_le_length_of_nodup_of_subset {α : Type} [DecidableEq α] (L M : List α)
   (hl : L.Nodup) (hsubset : L ⊆ M) : L.length ≤ M.length := by
   have h1 : L ⊆ M.dedup := by
     exact fun _ x ↦ List.subset_dedup M (hsubset x)
@@ -18,38 +20,35 @@ theorem nodup_subset_eq_length_le {α : Type} [DecidableEq α] (L M : List α)
     repeat assumption
   exact le_trans h3 h2
 
-theorem nodup_exists_mem_notMem_of_len_lt {α : Type} [DecidableEq α] (L M : List α)
+theorem exists_mem_notMem_of_nodup_of_len_lt {α : Type} [DecidableEq α] (L M : List α)
   (hl : L.Nodup) (hm : M.Nodup) (hlen : L.length < M.length) :
   ∃ x ∈ M, x ∉ L := by
   rw [← List.toFinset_card_of_nodup hl, ← List.toFinset_card_of_nodup hm] at hlen
   apply Finset.exists_mem_notMem_of_card_lt_card at hlen
   simp_all
 
-theorem count_gt_one_if {α : Type} [BEq α] [LawfulBEq α] (A : Array α) (n : Nat)
-  (h : A.size = n) (i j : Fin n) :
-  i ≠ j ∧ A[i] == A[j] → A.count (A[i]) > 1 := by
-  intro ⟨h1, h2⟩
-  simp_all [-Fin.getElem_fin]
+theorem one_lt_count {α : Type} [BEq α] [LawfulBEq α] (A : Array α)
+  (i j : Fin A.size) (h1 : i ≠ j) (h2 : A[i] == A[j]) :
+   1 < A.count (A[i]) := by
   apply Lean.Omega.Fin.lt_or_gt_of_ne at h1
+  rw [beq_iff_eq] at h2
   wlog h' : i < j generalizing i j
   · specialize this j i (Eq.symm h2) (by tauto) (by tauto)
-    rwa [h2] at this
-  have aux2 : Array.count A[j] (A.take j) ≥ 1 := by
-    simp [Array.mem_extract_iff_getElem]
+    rwa [← h2] at this
+  have aux1 : 1 ≤ Array.count A[j] (A.take j) := by
+    simp only [Array.take_eq_extract, Array.one_le_count_iff,
+    Array.mem_extract_iff_getElem]
     use i
-    simp
-    repeat constructor; assumption
-    rw [h]; exact i.isLt
-  have aux3 : Array.count A[j] (A.drop j) ≥ 1 := by
-    simp [Array.mem_extract_iff_getElem]
+    simp_all
+  have aux2 : 1 ≤ Array.count A[j] (A.drop j) := by
+    simp only [Array.drop_eq_extract, Array.one_le_count_iff,
+    Array.mem_extract_iff_getElem]
     use 0
     simp
-    rw [h]; exact j.isLt
   have : A.count A[j] = (A.take j ++ A.drop j).count A[j] := by
     congr
-    simp [j.isLt, h]
-    rw [← h]
-    simp only [Array.extract_size]
-  rw [this]
-  rw [Array.count_append]
+    simp_all [j.isLt, Array.extract_size]
+  rw [h2, this, Array.count_append]
   linarith
+
+end Aux
